examples/mutsum/MutMain1.v
@@ -1,0 +1,41 @@
+Require Import Coqlib.
+Require Import ITreelib.
+Require Import Universe.
+Require Import STS.
+Require Import Behavior.
+Require Import ModSem.
+Require Import Skeleton.
+Require Import PCM.
+Require Import Hoare.
+Require Import MutHeader.
+
+Generalizable Variables E R A B C X Y Σ.
+
+Set Implicit Arguments.
+
+
+
+Section PROOF.
+
+  Context `{Σ: GRA.t}.
+
+  Definition mainBody: list val -> itree (hCallE +' pE +' eventE) val :=
+    fun _ =>
+      trigger (hCall true "f" [Vint 10]↑);;
+      Ret (Vint 55)
+  .
+
+  Definition mainsbtb := [("main", mk_specbody main_spec mainBody)].
+
+  Definition mainSem: ModSem.t := {|
+    ModSem.fnsems := List.map (fun '(fn, body) => (fn, fun_to_tgt GlobalStb fn body)) mainsbtb;
+    ModSem.initial_mrs := [("Main", (ε, unit↑))];
+  |}
+  .
+
+  Definition main: Mod.t := {|
+    Mod.get_modsem := fun _ => mainSem;
+    Mod.sk := [("Main", Sk.Gfun)];
+  |}
+  .
+End PROOF.
